STLC/Smallstep.v
@@ -1,19 +1,22 @@
 Require Import Program.
-Require Import Syntax.
-
-Inductive value : Exp.t -> Prop :=
-  | V_Abs : forall e t, value (Exp.Abs t e).
-Hint Constructors value.
+Require Types Exp.
 
 Inductive simplto : Exp.t -> Exp.t -> Prop :=
   | S_AppL : forall e1 e1' e2,
       simplto e1 e1' ->
       simplto (Exp.App e1 e2) (Exp.App e1' e2)
   | S_AppR : forall v1 e2 e2',
-      value v1 ->
+      Exp.value v1 ->
       simplto e2 e2' ->
       simplto (Exp.App v1 e2) (Exp.App v1 e2')
   | S_App : forall e t v2,
-      value v2 ->
-      simplto (Exp.App (Exp.Abs t e) v2) (Exp.subst 0 [v2] e).
+      Exp.value v2 ->
+      simplto (Exp.App (Exp.Abs t e) v2) (Exp.subst 0 [v2] e)
+  | S_If : forall e1 e1' e2 e3,
+      simplto e1 e1' ->
+      simplto (Exp.If e1 e2 e3) (Exp.If e1' e2 e3)
+  | S_IfTrue : forall e2 e3,
+      simplto (Exp.If (Exp.Bool true) e2 e3) e2
+  | S_IfFalse : forall e2 e3,
+      simplto (Exp.If (Exp.Bool false) e2 e3) e3.
 Hint Constructors simplto.
