STLC/Normalize.v
@@ -1,27 +1,30 @@
 Require Import Arith List Program.
-Require Import Syntax Bigstep Typing.
+Require Import Types Exp Bigstep Typing.
 
 (* ugly definition... *)
 Fixpoint V t v : Prop :=
   match t with
-  | Types.Bool => False
+  | Types.Bool =>
+      exists b, v = Exp.Bool b
   | Types.Fun t1 t2 =>
       exists e,
       v = Exp.Abs t1 e /\ (forall v, V t1 v ->
-      (* exp t2 (Exp.subst 0 [v] e) *)
+      (* E t2 (Exp.subst 0 [v] e) *)
       exists v', evalto (Exp.subst 0 [v] e) v' /\ V t2 v')
   end.
 
+Definition E t e :=
+  exists v, evalto e v /\ V t v.
+
 Lemma V_impl_value : forall t v,
   V t v ->
-  value v.
+  Exp.value v.
 Proof.
   intros t v ?.
   destruct t; destruct v; simpl in *;
     repeat match goal with
     | H : exists _, _ |- _ => destruct H
     | H : _ /\ _ |- _ => destruct H
-    | H : False |- _ => destruct H
     end; solve [ congruence | auto ].
 Qed.
 Hint Resolve V_impl_value.
@@ -34,10 +37,11 @@ Lemma fundamental_property : forall env e t,
     nth i (map Some vs) None = Some v ->
     nth i (map Some env) None = Some t ->
     V t v) ->
-  exists v, evalto (Exp.subst 0 vs e) v /\ V t v.
+  E t (Exp.subst 0 vs e).
 Proof.
+  unfold E.
   intros ? ? ? Htyped.
-  induction Htyped; intros vs Hlength Henv; simpl in *.
+  induction Htyped; intros vs Hlength Henv; simpl in *; eauto.
   - rewrite Exp.shift_0 in *.
     rewrite <- minus_n_O in *.
     destruct (lt_dec x (length vs)).
@@ -51,7 +55,7 @@ Proof.
     + rewrite nth_overflow in * by (rewrite map_length; omega).
       discriminate.
   - eexists.
-    split; [ constructor |].
+    split; [ eauto |].
     eexists.
     split; [ reflexivity |].
     intros ? ?.
@@ -66,8 +70,11 @@ Proof.
     destruct (IHHtyped2 _ Hlength Henv) as [? [? HV]].
     destruct (Hsubst _ HV) as [? []].
     eauto.
+  - destruct (IHHtyped1 _ Hlength Henv) as [? [? [[]]]]; subst.
+    + destruct (IHHtyped2 _ Hlength Henv) as [? []]; eauto.
+    + destruct (IHHtyped3 _ Hlength Henv) as [? []]; eauto.
 Qed.
-            
+
 Lemma normalize : forall e t,
   typed [] e t ->
   exists v, evalto e v.
@@ -75,7 +82,8 @@ Proof.
   intros ? ? Htyped.
   apply fundamental_property with (vs := []) in Htyped; auto.
   - rewrite Exp.subst_nil in *.
-    destruct Htyped as [? []]; eauto.
+    destruct Htyped as [? []].
+    eauto.
   - intros i ? ? ? ?.
     destruct i; simpl in *; discriminate.
 Qed.
