STLC/Types.v
@@ -1,0 +1,3 @@
+Inductive t :=
+  | Bool
+  | Fun : t -> t -> t.
